theories/Refinement/Monads.v
@@ -28,7 +28,8 @@
 (******************************************************************************)
 
 From Coq Require Import
-     Classes.Morphisms.
+     Classes.Morphisms
+     Classes.Morphisms_Prop.
 From Equations Require Import
      Equations.
 From Katamaran Require Import
@@ -39,6 +40,7 @@ From Katamaran Require Import
      Symbolic.Propositions
      Symbolic.Solver
      Symbolic.Worlds
+     Syntax.Assertions
      Syntax.Chunks
      Syntax.Formulas
      Syntax.Predicates.
@@ -55,8 +57,9 @@ Module Type RefinementMonadsOn
   (Import SK : SolverKit B PK WR)
   (Import SP : SymPropOn B PK WR)
   (Import GS : GenericSolverOn B PK WR SK)
-  (Import SHAL : ShallowMonadsOn B PK WR SP)
-  (Import SYMB : SymbolicMonadsOn B PK WR SK SP GS).
+  (Import AS : AssertionsOn B PK WR)
+  (Import SHAL : ShallowMonadsOn B PK WR SP AS)
+  (Import SYMB : SymbolicMonadsOn B PK WR SK SP GS AS).
 
   Import ModalNotations logicalrelation logicalrelation.notations.
 
@@ -650,8 +653,6 @@ Module Type RefinementMonadsOn
       intros sΦ cΦ rΦ [HΦ]. revert HΦ. now apply rm.
     Qed.
 
-    #[local] Opaque RPureSpec.
-
     Lemma refine_assert_eq_nenv {N : Set} :
       ℛ⟦∀ Δ : NCtx N Ty, RMsg _ (RNEnv Δ -> RNEnv Δ -> RPureSpec RUnit)⟧
         SPureSpec.assert_eq_nenv CPureSpec.assert_eq_nenv.
@@ -685,7 +686,7 @@ Module Type RefinementMonadsOn
         SPureSpec.assert_eq_chunk CPureSpec.assert_eq_chunk.
     Proof.
       intros w0 ι0 Hpc0 msg c ? -> c' ? ->. revert c'.
-      induction c; intros [] w1 ω01 ι1 Hι1 Hpc1; cbn;
+      induction c; intros [] w1 ω01 ι1 Hι1 Hpc1; cbn - [RSat];
         auto; try (now apply refine_error).
       - destruct eq_dec.
         + destruct e; cbn.
@@ -710,8 +711,8 @@ Module Type RefinementMonadsOn
       ℛ⟦RInst (Sub Σ) (Valuation Σ) -> RPureSpec RUnit⟧
         (SPureSpec.replay_aux s) (CPureSpec.replay_aux s).
     Proof.
-      unfold RValid, RImpl. cbn.
-      induction s; cbn [SPureSpec.replay CPureSpec.replay];
+      unfold RValid, RImpl. cbn - [RPureSpec].
+      induction s; cbn [SPureSpec.replay_aux CPureSpec.replay_aux];
         intros w ι Hpc sδ cδ rδ.
       - apply refine_angelic_binary; auto.
       - apply refine_demonic_binary; auto.
@@ -780,6 +781,417 @@ Module Type RefinementMonadsOn
       cbn. now rewrite inst_sub_id.
     Qed.
 
+    Lemma refine_produce_chunk :
+      ℛ⟦RChunk -> RHeap -> RPureSpec RHeap⟧
+        SPureSpec.produce_chunk CPureSpec.produce_chunk.
+    Proof.
+      intros w ι Hpc sc cc rc sh ch rh.
+      unfold SPureSpec.produce_chunk, CPureSpec.produce_chunk.
+      apply refine_pure; auto. cbn.
+      rewrite peval_chunk_sound. now f_equal.
+    Qed.
+
+    Lemma refine_consume_chunk :
+      ℛ⟦RChunk -> RHeap -> RPureSpec RHeap⟧
+        SPureSpec.consume_chunk CPureSpec.consume_chunk.
+    Proof.
+      intros w0 ι0 Hpc0 cs cc -> sh ch ->.
+      unfold SPureSpec.consume_chunk.
+      set (c1 := peval_chunk cs).
+      destruct (try_consume_chunk_exact_spec sh c1) as [sh' HIn|].
+      { intros POST__s POST__c HPOST.
+        unfold CPureSpec.consume_chunk.
+        cbn. intros Hwp.
+        rewrite CPureSpec.wp_angelic_list.
+        change (SHeap w0) in sh'.
+        exists (inst c1 ι0, inst sh' ι0).
+        split.
+        - unfold inst at 3, inst_heap, inst_list.
+          rewrite heap_extractions_map, List.in_map_iff.
+          + exists (c1 , sh'). split. reflexivity. assumption.
+          + eauto using inst_is_duplicable.
+        - cbn. rewrite CPureSpec.wp_assert_eq_chunk. subst.
+          split; auto.
+          + subst c1. now rewrite peval_chunk_sound.
+          + revert Hwp. apply HPOST; now wsimpl.
+      }
+      destruct (try_consume_chunk_precise_spec sh c1) as [[sh' eqs] HIn|].
+      { cbv [SPureSpec.bind SPureSpec.pure].
+        intros POST__s POST__c HPOST.
+        match goal with | |- context[amsg.mk ?m] => generalize (amsg.mk m) end.
+        intros msg Hwp.
+        pose proof (refine_assert_pathcondition Hpc0 msg (ta := eqs)) as Hassert.
+        inster Hassert by (cbn; reflexivity).
+        match goal with
+        | H: SymProp.wsafe (SPureSpec.assert_pathcondition msg eqs ?P) _ |- _ =>
+            specialize (Hassert P (fun _ => POST__c (inst sh' ι0)))
+        end.
+        apply Hassert in Hwp; clear Hassert.
+        - destruct Hwp as [Heqs HP].
+          unfold CPureSpec.consume_chunk, CPureSpec.bind, CPureSpec.pure.
+          rewrite CPureSpec.wp_angelic_list.
+          exists (inst c1 ι0, inst sh' ι0). split; [auto|]. subst c1.
+          now rewrite CPureSpec.wp_assert_eq_chunk, peval_chunk_sound.
+        - intros w1 θ1 ι1 -> Hpc1 _ _ _. unfold T, four.
+          apply HPOST; auto.
+          + rewrite sub_acc_trans. cbn. now rewrite subst_sub_id.
+          + now eapply refine_inst_persist; eauto.
+      }
+      { intros POST__s POST__c HPOST. now apply refine_error. }
+    Qed.
+
+    Lemma refine_heap_extractions :
+      ℛ⟦RHeap -> RList (RProd RChunk RHeap)⟧
+        (fun w h => heap_extractions h)
+        (heap_extractions).
+    Proof.
+      intros w0 ι0 Hpc0 sh ch ->. hnf.
+      unfold inst, inst_heap, inst_list.
+      rewrite heap_extractions_map.
+      { clear. induction (heap_extractions sh) as [|[]];
+          cbn; constructor; cbn; auto. }
+      eauto using inst_is_duplicable.
+    Qed.
+
+    Lemma refine_consume_chunk_angelic :
+      ℛ⟦RChunk -> RHeap -> RPureSpec RHeap⟧
+        SPureSpec.consume_chunk_angelic CPureSpec.consume_chunk.
+    Proof.
+      intros w0 ι0 Hpc0 cs cc -> sh ch ->.
+      unfold SPureSpec.consume_chunk_angelic.
+      set (c1 := peval_chunk cs).
+      destruct (try_consume_chunk_exact_spec sh c1) as [sh' HIn|].
+      { intros POST__s POST__c HPOST.
+        unfold CPureSpec.consume_chunk.
+        cbn. intros Hwp.
+        rewrite CPureSpec.wp_angelic_list.
+        change (SHeap w0) in sh'.
+        exists (inst c1 ι0, inst sh' ι0).
+        split.
+        - unfold inst at 3, inst_heap, inst_list.
+          rewrite heap_extractions_map, List.in_map_iff.
+          + exists (c1 , sh'). split. reflexivity. assumption.
+          + eauto using inst_is_duplicable.
+        - cbn. rewrite CPureSpec.wp_assert_eq_chunk. subst.
+          split; auto.
+          + subst c1. now rewrite peval_chunk_sound.
+          + revert Hwp. apply HPOST; now wsimpl.
+      }
+      destruct (try_consume_chunk_precise_spec sh c1) as [[sh' eqs] HIn|].
+      { cbv [SPureSpec.bind SPureSpec.pure].
+        intros POST__s POST__c HPOST.
+        match goal with | |- context[amsg.mk ?m] => generalize (amsg.mk m) end.
+        intros msg Hwp.
+        pose proof (refine_assert_pathcondition Hpc0 msg (ta := eqs)) as Hassert.
+        inster Hassert by (cbn; reflexivity).
+        match goal with
+        | H: SymProp.wsafe (SPureSpec.assert_pathcondition msg eqs ?P) _ |- _ =>
+            specialize (Hassert P (fun _ => POST__c (inst sh' ι0)))
+        end.
+        apply Hassert in Hwp; clear Hassert.
+        - destruct Hwp as [Heqs HP].
+          unfold CPureSpec.consume_chunk, CPureSpec.bind, CPureSpec.pure.
+          rewrite CPureSpec.wp_angelic_list.
+          exists (inst c1 ι0, inst sh' ι0). split; [auto|]. subst c1.
+          now rewrite CPureSpec.wp_assert_eq_chunk, peval_chunk_sound.
+        - intros w1 θ1 ι1 -> Hpc1 _ _ _. unfold T, four.
+          apply HPOST; auto.
+          + rewrite sub_acc_trans. cbn. now rewrite subst_sub_id.
+          + now eapply refine_inst_persist; eauto.
+      }
+      { apply refine_bind; auto.
+        apply refine_angelic_list; auto.
+        now apply refine_heap_extractions.
+        intros w2 ω12 ι2 -> Hpc2.
+        intros [sc' sh'] [cc' ch'] [rc rh'].
+        apply refine_bind; auto.
+        - eapply refine_assert_eq_chunk; eauto.
+          + eapply refine_inst_persist; eauto.
+            subst c1. cbn.
+            now rewrite peval_chunk_sound.
+          + cbn. now rewrite inst_sub_id.
+        - intros w3 ω23 ι3 -> Hpc3 _ _ _.
+          apply refine_pure; auto.
+          eapply refine_inst_persist; eauto.
+      }
+    Qed.
+
+    Lemma refine_read_register {τ} (reg : 𝑹𝑬𝑮 τ) :
+      ℛ⟦RHeap -> RPureSpec (RProd (RVal τ) RHeap)⟧
+        (SPureSpec.read_register reg) (CPureSpec.read_register reg).
+    Proof.
+      unfold SPureSpec.read_register, SPureSpec.pure, T.
+      intros w0 ι0 Hpc0 sh ch -> sΦ cΦ rΦ HΦ.
+      destruct (find_chunk_ptsreg_precise_spec reg sh) as [[st sh'] HIn|].
+      - cbv [CPureSpec.read_register CPureSpec.consume_chunk CPureSpec.pure
+               CPureSpec.produce_chunk CPureSpec.bind CPureSpec.angelic].
+        set (v := inst (T := STerm τ) st ι0). exists v.
+        rewrite CPureSpec.wp_angelic_list.
+        exists (scchunk_ptsreg reg v, inst sh' ι0).
+        split. apply HIn.
+        rewrite CPureSpec.wp_assert_eq_chunk. split. easy.
+        revert HΦ. apply rΦ; cbn; auto.
+        now rewrite inst_sub_id.
+      - inversion HΦ.
+    Qed.
+
+    Lemma refine_write_register {τ} (reg : 𝑹𝑬𝑮 τ) :
+      ℛ⟦RVal τ -> RHeap -> RPureSpec (RProd (RVal τ) RHeap)⟧
+        (SPureSpec.write_register reg) (CPureSpec.write_register reg).
+    Proof.
+      unfold SPureSpec.write_register, SPureSpec.pure, T.
+      intros w0 ι0 Hpc0 sv cv rv sh ch rh sΦ cΦ rΦ HΦ.
+      destruct (find_chunk_ptsreg_precise_spec reg sh) as [[st sh'] HIn|].
+      - cbv [CPureSpec.write_register CPureSpec.consume_chunk CPureSpec.pure
+               CPureSpec.produce_chunk CPureSpec.bind CPureSpec.angelic].
+        set (vold := inst (T := STerm τ) st ι0). exists vold.
+        rewrite CPureSpec.wp_angelic_list.
+        exists (scchunk_ptsreg reg vold, inst sh' ι0).
+        split. rewrite rh. apply HIn.
+        rewrite CPureSpec.wp_assert_eq_chunk. split. easy.
+        revert HΦ. apply rΦ; auto.
+        + cbn. now rewrite inst_sub_id.
+        + constructor; auto. cbn. now do 2 f_equal.
+      - inversion HΦ.
+    Qed.
+
   End RPureSpec.
+
+  #[export] Instance RHeapSpec [SA CA] (RA : Rel SA CA) :
+    Rel (SHeapSpec SA) (CHeapSpec CA) := □(RA -> RHeap -> ℙ) -> RHeap -> ℙ.
+
+  Module RHeapSpec.
+
+    Lemma refine_run :
+      ℛ⟦RHeapSpec RUnit -> ℙ⟧ SHeapSpec.run CHeapSpec.run.
+    Proof. intros w0 ι0 Hpc0 sm cm rm. apply rm; constructor. Qed.
+
+    Lemma refine_lift_purespec `{RA : Rel SA CA} :
+      ℛ⟦RPureSpec RA -> RHeapSpec RA⟧
+        SHeapSpec.lift_purespec CHeapSpec.lift_purespec.
+    Proof.
+      unfold RPureSpec, RHeapSpec.
+      unfold SHeapSpec.lift_purespec, CHeapSpec.lift_purespec.
+      intros w ι Hpc ms mc Hm sΦ cΦ rΦ hs hc Hh. apply Hm.
+      intros w1 r01 ι1 Hι1 Hpc1 sa ca ra.
+      eapply refine_apply; eauto.
+      eapply refine_apply; eauto.
+      eapply refine_inst_persist; eauto.
+    Qed.
+
+    Lemma refine_pure `{RA : Rel SA CA} :
+      ℛ⟦RA -> RHeapSpec RA⟧ SHeapSpec.pure CHeapSpec.pure.
+    Proof.
+      intros w ι Hpc sv cv rv sΦ cΦ rΦ sh ch rh.
+      unfold SHeapSpec.pure, CHeapSpec.pure.
+      unfold CHeapSpec.lift_purespec, CPureSpec.pure.
+      eapply refine_apply; eauto.
+      eapply refine_apply; eauto.
+      apply refine_T; auto.
+    Qed.
+
+    Lemma refine_bind `{RA : Rel SA CA, RB : Rel SB CB} :
+      ℛ⟦RHeapSpec RA -> □(RA -> RHeapSpec RB) -> RHeapSpec RB⟧
+        SHeapSpec.bind CHeapSpec.bind.
+    Proof.
+      intros w0 ι0 Hpc0 sm cm rm sf cf rf sΦ cΦ rΦ sh ch rh.
+      unfold SHeapSpec.bind, CHeapSpec.bind. apply rm; auto.
+      intros w1 θ1 ι1 -> Hpc1 sa ca ra sh1 ch1 rh1.
+      apply rf; auto. eapply refine_four; eauto.
+    Qed.
+
+    Lemma refine_angelic x :
+      ℛ⟦∀ σ, RHeapSpec (RVal σ)⟧
+        (SHeapSpec.angelic x) (CHeapSpec.angelic).
+    Proof.
+      intros w0 ι0 Hpc0 σ.
+      apply refine_lift_purespec; auto.
+      apply RPureSpec.refine_angelic; auto.
+    Qed.
+
+    Lemma refine_demonic x :
+      ℛ⟦∀ σ, RHeapSpec (RVal σ)⟧
+        (SHeapSpec.demonic x) (CHeapSpec.demonic).
+    Proof.
+      intros w0 ι0 Hpc0 σ.
+      apply refine_lift_purespec; auto.
+      apply RPureSpec.refine_demonic; auto.
+    Qed.
+
+    Lemma refine_angelic_binary `{RA : Rel SA CA} :
+      ℛ⟦RHeapSpec RA -> RHeapSpec RA -> RHeapSpec RA⟧
+        SHeapSpec.angelic_binary CHeapSpec.angelic_binary.
+    Proof.
+      intros w0 ι0 Hpc0 sm1 cm1 rm1 sm2 cm2 rm2 sΦ cΦ rΦ sh ch rh.
+      cbn. apply or_impl_morphism. now apply rm1. now apply rm2.
+    Qed.
+
+    Lemma refine_demonic_binary `{RA : Rel SA CA} :
+      ℛ⟦RHeapSpec RA -> RHeapSpec RA -> RHeapSpec RA⟧
+        SHeapSpec.demonic_binary CHeapSpec.demonic_binary.
+    Proof.
+      intros w0 ι0 Hpc0 sm1 cm1 rm1 sm2 cm2 rm2 sΦ cΦ rΦ sh ch rh.
+      cbn. apply and_impl_morphism. now apply rm1. now apply rm2.
+    Qed.
+
+    Lemma refine_debug `{RA : Rel SA CA} :
+      ℛ⟦RMsg _ (RHeapSpec RA -> RHeapSpec RA)⟧
+        SHeapSpec.debug CHeapSpec.debug.
+    Proof.
+      intros w0 ι0 Hpc0 msg sm cm rm sΦ cΦ rΦ sh ch rh.
+      intros [HΦ]. revert HΦ. now apply rm.
+    Qed.
+
+    Lemma refine_assert_formula :
+      ℛ⟦RMsg _ (RFormula -> RHeapSpec RUnit)⟧
+        SHeapSpec.assert_formula CHeapSpec.assert_formula.
+    Proof.
+      intros w0 ι0 Hpc0 msg sF cF rF sΦ cΦ rΦ sh ch rh.
+      apply RPureSpec.refine_assert_formula; auto.
+      intros w1 θ1 ι1 Hι1 Hpc1 su cu ru. apply rΦ; auto.
+      eapply refine_inst_persist; eauto.
+    Qed.
+
+    Lemma refine_assume_formula :
+      ℛ⟦RFormula -> RHeapSpec RUnit⟧
+        SHeapSpec.assume_formula CHeapSpec.assume_formula.
+    Proof.
+      intros w0 ι0 Hpc0 msg sF cF rF.
+      apply refine_lift_purespec; auto.
+      apply RPureSpec.refine_assume_formula; auto.
+    Qed.
+
+    Lemma refine_produce_chunk :
+      ℛ⟦RChunk -> RHeapSpec RUnit⟧
+        SHeapSpec.produce_chunk CHeapSpec.produce_chunk.
+    Proof.
+      intros w0 ι0 Hpc0 sc cc rc sΦ cΦ rΦ sh ch rh.
+      unfold SHeapSpec.produce_chunk.
+      unfold CHeapSpec.produce_chunk.
+      apply RPureSpec.refine_produce_chunk; auto.
+      intros w1 θ1 ι1 Hι1 Hpc1. now apply rΦ.
+    Qed.
+
+    Lemma refine_consume_chunk :
+      ℛ⟦RChunk -> RHeapSpec RUnit⟧
+        SHeapSpec.consume_chunk CHeapSpec.consume_chunk.
+    Proof.
+      intros w0 ι0 Hpc0 sc cc rc sΦ cΦ rΦ sh ch rh.
+      unfold SHeapSpec.consume_chunk.
+      unfold CHeapSpec.consume_chunk.
+      apply RPureSpec.refine_consume_chunk; auto.
+      intros w1 θ1 ι1 Hι1 Hpc1. now apply rΦ.
+    Qed.
+
+    Lemma refine_consume_chunk_angelic :
+      ℛ⟦RChunk -> RHeapSpec RUnit⟧
+        SHeapSpec.consume_chunk_angelic CHeapSpec.consume_chunk.
+    Proof.
+      intros w0 ι0 Hpc0 sc cc rc sΦ cΦ rΦ sh ch rh.
+      unfold SHeapSpec.consume_chunk_angelic.
+      unfold CHeapSpec.consume_chunk.
+      apply RPureSpec.refine_consume_chunk_angelic; auto.
+      intros w1 θ1 ι1 Hι1 Hpc1. now apply rΦ.
+    Qed.
+
+    Lemma refine_produce {Σ} (asn : Assertion Σ) :
+      ℛ⟦RInst (Sub Σ) (Valuation Σ) -> RHeapSpec RUnit⟧
+        (SHeapSpec.produce asn) (CHeapSpec.produce asn).
+    Proof.
+      induction asn; intros w0 ι0 Hpc0 sδ cδ rδ; cbn - [RSat].
+      - apply refine_assume_formula; auto.
+        now apply refine_formula_subst.
+      - apply refine_produce_chunk; eauto.
+        hnf. now rewrite inst_subst, rδ.
+      - apply refine_produce_chunk; eauto.
+        hnf. now rewrite inst_subst, rδ.
+      - apply refine_bind; auto.
+        apply refine_lift_purespec; auto.
+        apply RPureSpec.refine_demonic_pattern_match; auto.
+        hnf. now rewrite inst_subst, rδ.
+        intros w1 θ1 ι1 -> Hpc1 [] [] []. subst. cbn in H0. subst.
+        eapply H; eauto. hnf. hnf in rδ. subst.
+        symmetry. etransitivity.
+        refine (inst_env_cat (persist sδ θ1) n ι1).
+        f_equal. apply inst_persist.
+      - apply refine_bind; auto.
+        apply IHasn1; auto.
+        intros w1 θ1 ι1 Hι1 Hpc1 _ _ _.
+        apply IHasn2; auto.
+        eapply refine_inst_persist; eauto.
+      - eapply refine_demonic_binary; eauto.
+        apply IHasn1; auto. apply IHasn2; auto.
+      - eapply refine_bind; auto.
+        apply refine_lift_purespec; auto.
+        apply RPureSpec.refine_demonic; auto.
+        intros w1 θ1 ι1 -> Hpc1 sv cv ->.
+        apply IHasn; auto.
+        cbn - [inst]. cbn in rδ. subst.
+        now rewrite <- inst_persist.
+      - apply refine_debug; auto.
+        apply refine_pure; auto.
+        constructor.
+    Qed.
+
+    Lemma refine_consume {Σ} (asn : Assertion Σ) :
+      ℛ⟦RInst (Sub Σ) (Valuation Σ) -> RHeapSpec RUnit⟧
+        (SHeapSpec.consume asn) (CHeapSpec.consume asn).
+    Proof.
+      induction asn; intros w0 ι0 Hpc0 sδ cδ rδ; cbn - [RSat].
+      - apply refine_assert_formula; auto.
+        now apply refine_formula_subst.
+      - apply refine_consume_chunk; eauto.
+        hnf. now rewrite inst_subst, rδ.
+      - apply refine_consume_chunk_angelic; eauto.
+        hnf. now rewrite inst_subst, rδ.
+      - apply refine_bind; auto.
+        apply refine_lift_purespec; auto.
+        apply RPureSpec.refine_angelic_pattern_match; auto.
+        hnf. now rewrite inst_subst, rδ.
+        intros w1 θ1 ι1 -> Hpc1 [] [] []. subst. cbn in H0. subst.
+        eapply H; eauto. hnf. hnf in rδ. subst.
+        symmetry. etransitivity.
+        refine (inst_env_cat (persist sδ θ1) n ι1).
+        f_equal. apply inst_persist.
+      - apply refine_bind; auto.
+        apply IHasn1; auto.
+        intros w1 θ1 ι1 Hι1 Hpc1 _ _ _.
+        apply IHasn2; auto.
+        eapply refine_inst_persist; eauto.
+      - eapply refine_angelic_binary; eauto.
+        apply IHasn1; auto. apply IHasn2; auto.
+      - eapply refine_bind; auto.
+        apply refine_lift_purespec; auto.
+        apply RPureSpec.refine_angelic; auto.
+        intros w1 θ1 ι1 -> Hpc1 sv cv ->.
+        apply IHasn; auto.
+        cbn - [inst]. cbn in rδ. subst.
+        now rewrite <- inst_persist.
+      - apply refine_debug; auto.
+        apply refine_pure; auto.
+        constructor.
+    Qed.
+
+    Lemma refine_read_register {τ} (reg : 𝑹𝑬𝑮 τ) :
+      ℛ⟦RHeapSpec (RVal τ)⟧
+        (@SHeapSpec.read_register _ reg) (CHeapSpec.read_register reg).
+    Proof.
+      intros w0 ι0 Hpc0 sΦ cΦ rΦ sh ch rh.
+      apply RPureSpec.refine_read_register; auto.
+      intros w1 θ1 ι1 Hι1 Hpc1 [sv sh'] [cv ch'] [rv rh'].
+      now apply rΦ.
+    Qed.
+
+    Lemma refine_write_register {τ} (reg : 𝑹𝑬𝑮 τ) :
+      ℛ⟦RVal τ -> RHeapSpec (RVal τ)⟧
+        (@SHeapSpec.write_register _ reg) (CHeapSpec.write_register reg).
+    Proof.
+      intros w0 ι0 Hpc0 sv cv rv sΦ cΦ rΦ sh ch rh.
+      apply RPureSpec.refine_write_register; auto.
+      intros w1 θ1 ι1 Hι1 Hpc1 [sv' sh'] [cv' ch'] [rv' rh'].
+      now apply rΦ.
+    Qed.
+
+  End RHeapSpec.
 
 End RefinementMonadsOn.
